theories/simplang/heapbij_refl.v
@@ -1,6 +1,6 @@
 From simuliris.simulation Require Import slsls lifting.
 From simuliris.simplang Require Import proofmode tactics.
-From simuliris.simplang Require Import parallel_subst heap_bij open_expr_rel.
+From simuliris.simplang Require Import parallel_subst heap_bij log_rel.
 
 (** * Reflexivity theorem for the heap bijection value relation *)
 
@@ -110,15 +110,15 @@ Section refl.
     sim_bind ctx_t ctx_s;
     iApply (sim_wand with Hp).
 
-  Lemma expr_rel_var x : ⊢ expr_rel (Var x) (Var x).
+  Lemma log_rel_var x : ⊢ log_rel (Var x) (Var x).
   Proof.
     iIntros (? xs) "!# #Hs"; simpl.
     iDestruct (subst_map_rel_lookup x with "Hs") as (v_t v_s Hv) "Hrel"; first set_solver.
     rewrite !lookup_fmap Hv /=. sim_val. done.
   Qed.
 
-  Lemma expr_rel_let x e1_t e1_s e2_t e2_s :
-    expr_rel e1_t e1_s -∗ expr_rel e2_t e2_s -∗ expr_rel (Let x e1_t e2_t) (Let x e1_s e2_s).
+  Lemma log_rel_let x e1_t e1_s e2_t e2_s :
+    log_rel e1_t e1_s -∗ log_rel e2_t e2_s -∗ log_rel (Let x e1_t e2_t) (Let x e1_s e2_s).
   Proof.
     iIntros "#IH1 #IH2" (? xs) "!# #Hs"; simpl.
     smart_sim_bind (subst_map _ _) (subst_map _ _) "(IH1 [])".
@@ -134,8 +134,8 @@ Section refl.
     destruct (decide (x = x')) as [<-|Hne]; set_solver.
   Qed.
 
-  Lemma expr_rel_call e1_t e1_s e2_t e2_s :
-    expr_rel e1_t e1_s -∗ expr_rel e2_t e2_s -∗ expr_rel (Call e1_t e2_t) (Call e1_s e2_s).
+  Lemma log_rel_call e1_t e1_s e2_t e2_s :
+    log_rel e1_t e1_s -∗ log_rel e2_t e2_s -∗ log_rel (Call e1_t e2_t) (Call e1_s e2_s).
   Proof.
     iIntros "#IH1 #IH2" (? xs) "!# #Hs"; simpl.
     smart_sim_bind (subst_map _ _) (subst_map _ _) "(IH2 [])".
@@ -148,8 +148,8 @@ Section refl.
     iApply sim_call; done.
   Qed.
 
-  Lemma expr_rel_unop e_t e_s o :
-    expr_rel e_t e_s -∗ expr_rel (UnOp o e_t) (UnOp o e_s).
+  Lemma log_rel_unop e_t e_s o :
+    log_rel e_t e_s -∗ log_rel (UnOp o e_t) (UnOp o e_s).
   Proof.
     iIntros "#IH" (? xs) "!# #Hs"; simpl.
     smart_sim_bind (subst_map _ e_t) (subst_map _ e_s) "(IH [])".
@@ -158,8 +158,8 @@ Section refl.
     destruct o; sim_pures; discr_source; val_discr_source "Hv"; by sim_pures; sim_val.
   Qed.
 
-  Lemma expr_rel_binop e1_t e1_s e2_t e2_s o :
-    expr_rel e1_t e1_s -∗ expr_rel e2_t e2_s -∗ expr_rel (BinOp o e1_t e2_t) (BinOp o e1_s e2_s).
+  Lemma log_rel_binop e1_t e1_s e2_t e2_s o :
+    log_rel e1_t e1_s -∗ log_rel e2_t e2_s -∗ log_rel (BinOp o e1_t e2_t) (BinOp o e1_s e2_s).
   Proof.
     iIntros "#IH1 #IH2" (? xs) "!# #Hs"; simpl.
     smart_sim_bind (subst_map _ e2_t) (subst_map _ e2_s) "(IH2 [])".
@@ -184,11 +184,11 @@ Section refl.
       by iApply heap_bij_loc_shift.
   Qed.
 
-  Lemma expr_rel_if e1_t e1_s e2_t e2_s e3_t e3_s :
-    expr_rel e1_t e1_s -∗
-    expr_rel e2_t e2_s -∗
-    expr_rel e3_t e3_s -∗
-    expr_rel (If e1_t e2_t e3_t) (If e1_s e2_s e3_s).
+  Lemma log_rel_if e1_t e1_s e2_t e2_s e3_t e3_s :
+    log_rel e1_t e1_s -∗
+    log_rel e2_t e2_s -∗
+    log_rel e3_t e3_s -∗
+    log_rel (If e1_t e2_t e3_t) (If e1_s e2_s e3_s).
   Proof.
     iIntros "#IH1 #IH2 #IH3" (? xs) "!# #Hs"; simpl.
     smart_sim_bind (subst_map _ e1_t) (subst_map _ e1_s) "(IH1 [])".
@@ -199,10 +199,10 @@ Section refl.
     + iApply "IH3". iApply (subst_map_rel_weaken with "[$]"). set_solver.
   Qed.
 
-  Lemma expr_rel_while e1_t e1_s e2_t e2_s :
-    expr_rel e1_t e1_s -∗
-    expr_rel e2_t e2_s -∗
-    expr_rel (While e1_t e2_t) (While e1_s e2_s).
+  Lemma log_rel_while e1_t e1_s e2_t e2_s :
+    log_rel e1_t e1_s -∗
+    log_rel e2_t e2_s -∗
+    log_rel (While e1_t e2_t) (While e1_s e2_s).
   Proof.
     iIntros "#IH1 #IH2" (? xs) "!# #Hs"; simpl.
     iApply (sim_while_while _ _ _ _ _ _ (True)%I with "[//]").
@@ -217,10 +217,10 @@ Section refl.
     + iApply sim_expr_base. iLeft. iExists #(), #(); eauto.
   Qed.
 
-  Lemma expr_rel_pair e1_t e1_s e2_t e2_s :
-    expr_rel e1_t e1_s -∗
-    expr_rel e2_t e2_s -∗
-    expr_rel (Pair e1_t e2_t) (Pair e1_s e2_s).
+  Lemma log_rel_pair e1_t e1_s e2_t e2_s :
+    log_rel e1_t e1_s -∗
+    log_rel e2_t e2_s -∗
+    log_rel (Pair e1_t e2_t) (Pair e1_s e2_s).
   Proof.
     iIntros "#IH1 #IH2" (? xs) "!# #Hs"; simpl.
     smart_sim_bind (subst_map _ e2_t) (subst_map _ e2_s) "(IH2 [])".
@@ -232,8 +232,8 @@ Section refl.
     sim_pures; sim_val. iModIntro; iSplit; eauto.
   Qed.
 
-  Lemma expr_rel_fst e_t e_s :
-    expr_rel e_t e_s -∗ expr_rel (Fst e_t) (Fst e_s).
+  Lemma log_rel_fst e_t e_s :
+    log_rel e_t e_s -∗ log_rel (Fst e_t) (Fst e_s).
   Proof.
     iIntros "#IH" (? xs) "!# #Hs"; simpl.
     smart_sim_bind (subst_map _ e_t) (subst_map _ e_s) "(IH [])".
@@ -242,8 +242,8 @@ Section refl.
     discr_source.
     iPoseProof (val_rel_pair_source with "Hv") as (??) "(-> & ? & ?)"; by sim_pures; sim_val.
   Qed.
-  Lemma expr_rel_snd e_t e_s :
-    expr_rel e_t e_s -∗ expr_rel (Snd e_t) (Snd e_s).
+  Lemma log_rel_snd e_t e_s :
+    log_rel e_t e_s -∗ log_rel (Snd e_t) (Snd e_s).
   Proof.
     iIntros "#IH" (? xs) "!# #Hs"; simpl.
     smart_sim_bind (subst_map _ e_t) (subst_map _ e_s) "(IH [])".
@@ -253,16 +253,16 @@ Section refl.
     iPoseProof (val_rel_pair_source with "Hv") as (??) "(-> & ? & ?)"; by sim_pures; sim_val.
   Qed.
 
-  Lemma expr_rel_injl e_t e_s :
-    expr_rel e_t e_s -∗ expr_rel (InjL e_t) (InjL e_s).
+  Lemma log_rel_injl e_t e_s :
+    log_rel e_t e_s -∗ log_rel (InjL e_t) (InjL e_s).
   Proof.
     iIntros "#IH" (? xs) "!# #Hs"; simpl.
     smart_sim_bind (subst_map _ e_t) (subst_map _ e_s) "(IH [])".
     { iApply (subst_map_rel_weaken with "[$]"). set_solver. }
     iIntros (v_t v_s) "Hv"; by sim_pures; sim_val.
   Qed.
-  Lemma expr_rel_injr e_t e_s :
-    expr_rel e_t e_s -∗ expr_rel (InjR e_t) (InjR e_s).
+  Lemma log_rel_injr e_t e_s :
+    log_rel e_t e_s -∗ log_rel (InjR e_t) (InjR e_s).
   Proof.
     iIntros "#IH" (? xs) "!# #Hs"; simpl.
     smart_sim_bind (subst_map _ e_t) (subst_map _ e_s) "(IH [])".
@@ -270,11 +270,11 @@ Section refl.
     iIntros (v_t v_s) "Hv"; by sim_pures; sim_val.
   Qed.
 
-  Lemma expr_rel_match e_t e_s e1_t e1_s e2_t e2_s x1 x2 :
-    expr_rel e_t e_s -∗
-    expr_rel e1_t e1_s -∗
-    expr_rel e2_t e2_s -∗
-    expr_rel (Match e_t x1 e1_t x2 e2_t) (Match e_s x1 e1_s x2 e2_s).
+  Lemma log_rel_match e_t e_s e1_t e1_s e2_t e2_s x1 x2 :
+    log_rel e_t e_s -∗
+    log_rel e1_t e1_s -∗
+    log_rel e2_t e2_s -∗
+    log_rel (Match e_t x1 e1_t x2 e2_t) (Match e_s x1 e1_s x2 e2_s).
   Proof.
     iIntros "#IH #IH1 #IH2" (? xs) "!# #Hs"; simpl.
     smart_sim_bind (subst_map _ e_t) (subst_map _ e_s)  "(IH [])".
@@ -303,16 +303,16 @@ Section refl.
       destruct (decide (x2 = x')) as [<-|Hne]; set_solver.
   Qed.
 
-  Lemma expr_rel_fork e_t e_s :
-    expr_rel e_t e_s -∗ expr_rel (Fork e_t) (Fork e_s).
+  Lemma log_rel_fork e_t e_s :
+    log_rel e_t e_s -∗ log_rel (Fork e_t) (Fork e_s).
   Proof.
     iIntros "#IH" (? xs) "!# #Hs"; simpl.
     iApply sim_fork; first by sim_pures; sim_val. iIntros (?). sim_pures.
     iApply (sim_wand with "(IH [])"); eauto.
   Qed.
 
-  Lemma expr_rel_allocN e1_t e1_s e2_t e2_s :
-    expr_rel e1_t e1_s -∗ expr_rel e2_t e2_s -∗ expr_rel (AllocN e1_t e2_t) (AllocN e1_s e2_s).
+  Lemma log_rel_allocN e1_t e1_s e2_t e2_s :
+    log_rel e1_t e1_s -∗ log_rel e2_t e2_s -∗ log_rel (AllocN e1_t e2_t) (AllocN e1_s e2_s).
   Proof.
     iIntros "#IH1 #IH2" (? xs) "!# #Hs"; simpl.
     smart_sim_bind (subst_map _ e2_t) (subst_map _ e2_s) "(IH2 [])".
@@ -333,8 +333,8 @@ Section refl.
     iIntros "Hv". sim_pures. sim_val. done.
   Qed.
 
-  Lemma expr_rel_freeN e1_t e1_s e2_t e2_s :
-    expr_rel e1_t e1_s -∗ expr_rel e2_t e2_s -∗ expr_rel (FreeN e1_t e2_t) (FreeN e1_s e2_s).
+  Lemma log_rel_freeN e1_t e1_s e2_t e2_s :
+    log_rel e1_t e1_s -∗ log_rel e2_t e2_s -∗ log_rel (FreeN e1_t e2_t) (FreeN e1_s e2_s).
   Proof.
     iIntros "#IH1 #IH2" (? xs) "!# #Hs"; simpl.
     smart_sim_bind (subst_map _ _) (subst_map _ _) "(IH2 [])".
@@ -348,8 +348,8 @@ Section refl.
     by sim_free; sim_val.
   Qed.
 
-  Lemma expr_rel_load o e_t e_s :
-    expr_rel e_t e_s -∗ expr_rel (Load o e_t) (Load o e_s).
+  Lemma log_rel_load o e_t e_s :
+    log_rel e_t e_s -∗ log_rel (Load o e_t) (Load o e_s).
   Proof.
     iIntros "#IH" (? xs) "!# #Hs"; simpl.
     smart_sim_bind (subst_map _ _) (subst_map _ _) "(IH [])".
@@ -358,8 +358,8 @@ Section refl.
     by sim_load v_t v_s as "Hv"; sim_val.
   Qed.
 
-  Lemma expr_rel_store o e1_t e1_s e2_t e2_s :
-    expr_rel e1_t e1_s -∗ expr_rel e2_t e2_s -∗ expr_rel (Store o e1_t e2_t) (Store o e1_s e2_s).
+  Lemma log_rel_store o e1_t e1_s e2_t e2_s :
+    log_rel e1_t e1_s -∗ log_rel e2_t e2_s -∗ log_rel (Store o e1_t e2_t) (Store o e1_s e2_s).
   Proof.
     iIntros "#IH1 #IH2" (? xs) "!# #Hs"; simpl.
     smart_sim_bind (subst_map _ _) (subst_map _ _) "(IH2 [])".
@@ -372,33 +372,33 @@ Section refl.
     by sim_store; [done | sim_val].
   Qed.
 
-  Lemma expr_rel_val v_t v_s :
-    val_rel v_t v_s -∗ expr_rel (Val v_t) (Val v_s).
+  Lemma log_rel_val v_t v_s :
+    val_rel v_t v_s -∗ log_rel (Val v_t) (Val v_s).
   Proof. iIntros "#Hv" (? xs) "!# #Hs"; simpl. by sim_val. Qed.
 
-  Theorem expr_wf_sound e : expr_wf e → ⊢ expr_rel e e.
+  Theorem expr_wf_sound e : expr_wf e → ⊢ log_rel e e.
   Proof.
     intros Hwf. iInduction e as [ ] "IH" forall (Hwf); iIntros (? xs) "!# #Hs"; simpl.
-    - (* Val *) iApply expr_rel_val; [by iApply val_wf_sound | done].
-    - (* Var *) by iApply expr_rel_var.
-    - (* Let *) destruct Hwf as [Hwf1 Hwf2]. by iApply (expr_rel_let with "(IH [//]) (IH1 [//])").
-    - (* Call *) destruct Hwf as [Hwf1 Hwf2]. by iApply (expr_rel_call with "(IH [//]) (IH1 [//])").
-    - (* UnOp *) by iApply (expr_rel_unop with "(IH [//])").
-    - (* BinOp *) destruct Hwf as [Hwf1 Hwf2]. by iApply (expr_rel_binop with "(IH [//]) (IH1 [//])").
-    - (* If *) destruct Hwf as (Hwf1 & Hwf2 & Hwf3). by iApply (expr_rel_if with "(IH [//]) (IH1 [//]) (IH2 [//])").
-    - (* While *) destruct Hwf as (Hwf1 & Hwf2). by iApply (expr_rel_while with "(IH [//]) (IH1 [//])").
-    - (* Pairs *) destruct Hwf as (Hwf1 & Hwf2). by iApply (expr_rel_pair with "(IH [//]) (IH1 [//])").
-    - (* Fst *) by iApply (expr_rel_fst with "(IH [//])").
-    - (* Snd *) by iApply (expr_rel_snd with "(IH [//])").
-    - (* InjL *) by iApply (expr_rel_injl with "(IH [//])").
-    - (* InjR *) by iApply (expr_rel_injr with "(IH [//])").
+    - (* Val *) iApply log_rel_val; [by iApply val_wf_sound | done].
+    - (* Var *) by iApply log_rel_var.
+    - (* Let *) destruct Hwf as [Hwf1 Hwf2]. by iApply (log_rel_let with "(IH [//]) (IH1 [//])").
+    - (* Call *) destruct Hwf as [Hwf1 Hwf2]. by iApply (log_rel_call with "(IH [//]) (IH1 [//])").
+    - (* UnOp *) by iApply (log_rel_unop with "(IH [//])").
+    - (* BinOp *) destruct Hwf as [Hwf1 Hwf2]. by iApply (log_rel_binop with "(IH [//]) (IH1 [//])").
+    - (* If *) destruct Hwf as (Hwf1 & Hwf2 & Hwf3). by iApply (log_rel_if with "(IH [//]) (IH1 [//]) (IH2 [//])").
+    - (* While *) destruct Hwf as (Hwf1 & Hwf2). by iApply (log_rel_while with "(IH [//]) (IH1 [//])").
+    - (* Pairs *) destruct Hwf as (Hwf1 & Hwf2). by iApply (log_rel_pair with "(IH [//]) (IH1 [//])").
+    - (* Fst *) by iApply (log_rel_fst with "(IH [//])").
+    - (* Snd *) by iApply (log_rel_snd with "(IH [//])").
+    - (* InjL *) by iApply (log_rel_injl with "(IH [//])").
+    - (* InjR *) by iApply (log_rel_injr with "(IH [//])").
     - (* Match *) destruct Hwf as (Hwf1 & Hwf2 & Hwf3).
-      by iApply (expr_rel_match with "(IH [//]) (IH1 [//]) (IH2 [//])").
-    - (* Fork *) by iApply (expr_rel_fork with "(IH [//])").
-    - (* AllocN *) destruct Hwf as (Hwf1 & Hwf2). by iApply (expr_rel_allocN with "(IH [//]) (IH1 [//])").
-    - (* FreeN *) destruct Hwf as (Hwf1 & Hwf2). by iApply (expr_rel_freeN with "(IH [//]) (IH1 [//])").
-    - (* Load *) by iApply (expr_rel_load with "(IH [//])").
-    - (* Store *) destruct Hwf as (Hwf1 & Hwf2). by iApply (expr_rel_store with "(IH [//]) (IH1 [//])").
+      by iApply (log_rel_match with "(IH [//]) (IH1 [//]) (IH2 [//])").
+    - (* Fork *) by iApply (log_rel_fork with "(IH [//])").
+    - (* AllocN *) destruct Hwf as (Hwf1 & Hwf2). by iApply (log_rel_allocN with "(IH [//]) (IH1 [//])").
+    - (* FreeN *) destruct Hwf as (Hwf1 & Hwf2). by iApply (log_rel_freeN with "(IH [//]) (IH1 [//])").
+    - (* Load *) by iApply (log_rel_load with "(IH [//])").
+    - (* Store *) destruct Hwf as (Hwf1 & Hwf2). by iApply (log_rel_store with "(IH [//]) (IH1 [//])").
     - done.
     - done.
   Qed.
